<script type="text/x-mathjax-config">
  MathJax.Hub.Config({
    tex2jax: {
      inlineMath: [ ['$','$'], ["\\(","\\)"] ],
      processEscapes: true
    }
  });
</script>

<script type="text/javascript" async
  src="https://cdnjs.cloudflare.com/ajax/libs/mathjax/2.7.5/MathJax.js?config=TeX-MML-AM_CHTML">
</script>
<script type="text/javascript" src="tutorialSheetScripts.js"> </script>
<link rel="stylesheet" type="text/css" media="all" href="styles.css">

![function](01-refersher-and-functions-media/cover.png)
# Refresher and Functions Tutorial Sheet, Sheet #1

### Learning Targets

1. Use the method of partial fractions
1. Find the derivative of functions with the product, chain and sum rules
1. Find the integral of functions using the power rule, sum rule and integration by parts
1. Simplify logarithms
1. Identify key points in a function (roots, asymptotes, stationary points, inflection points, domain, range)
1. Sketch a graph of a given function

<!-- ### Reading
* [Intro](https://legoyoda112.github.io/DE-MEM-Resources/files/DE1-MEM_notes_2019.pdf#page=7)
* [Chapter 0 - Refersher](https://legoyoda112.github.io/DE-MEM-Resources/files/DE1-MEM_notes_2019.pdf#page=10)
* [Chapter 1 - Functions](https://legoyoda112.github.io/DE-MEM-Resources/files/DE1-MEM_notes_2019.pdf#page=18)

### Lectures
* Welcome (monday) *(populate with recording link?)*
* Function sketching (tuesday) * -->

### Additional Resources
* [SJC - Curve Sketching](https://youtu.be/EFxv2r9gwtc)
* [3Blue1Brown - Calculus Playlist](https://www.youtube.com/playlist?list=PLZHQObOWTQDMsr9K-rj53DwVRMYO3t5Yr)
* [WA - Sketch Any Function](https://www.wolframalpha.com/input/?i=(x%5E2%2B3x-7)%2F(x-9))

<br><br><br><br>


# Problem sheet
## Essential Questions
### Problem 1.
Separate the following using the method of partial fractions.

(a) $\frac{x^2-6}{x^3-x}$
<div class = "answer">$\Rightarrow \quad $ factorise the denominator $\Rightarrow{}\ \ x^3-x = x(x+1)(x-1)$ <br>
$\Rightarrow{}\ \ \frac{x^2-6}{x^3-x} = \frac{A}{x} + \frac{B}{(x+1)} + \frac{C}{(x-1)}$ <br>
from numerators  $x^2 - 6 = (A+B+C)x^2 + (C-B)x - A$ <br>
$\Rightarrow \quad A+B+C = 1,\\ \quad C-B = 0,\\ \quad A = 6$ <br>
$\Rightarrow \quad C = B = \frac{-5}{2}$ <br>
$\Rightarrow{}\ \ \boxed{ \frac{x^2-6}{x^3-x} = \frac{6}{x} - \frac{5}{2(x+1)} - \frac{5}{2(x-1)}}$
</div>

(b) $\frac{5(x-7)}{x^2+2x-35}$
<div class = "answer">$\Rightarrow{}\quad$ factorize the denominator <br>
$\Rightarrow \quad x^2+2x-35 = (x+7)(x-5)$ <br>
$\Rightarrow \quad \frac{5(x-7)}{x^2+2x-35} = \frac{A}{x+7} + \frac{B}{x-5}$ <br>
$\Rightarrow \quad $ from numerators  $5x-35 = (A+B)x - 5A + 7B$ <br>
$\Rightarrow \quad A+B = 5,\quad -5A + 7B = -35$ <br>
$\Rightarrow \quad \boxed{A = \frac{35}{6},\quad B=\frac{-5}{6},
\ \ \frac{5(x-7)}{x^2+2x-35} = \frac{35}{6(x+7)} - \frac{5}{6(x-5)} }$
</div>

(c) $\frac{x-1}{(3x+2)^2(2x+3)}$
<div class = "answer">$\Rightarrow{}\quad$ for linear and repeated factors <br>
$\Rightarrow{}\ \ \frac{x-1}{(3x+2)^2(2x+3)} = \frac{A}{2x+3} + \frac{B}{3x+2} + \frac{C}{(3x+2)^2}$ <br>
$\Rightarrow{}\quad$from numerators $\Rightarrow{}\quad x-1 = (9A+6B)x^2 + (12A+13B+2C)x + 4A + 6B +3C$ <br>
$\Rightarrow{}\quad 9A+6B = 0,\quad 12A +13B +2C = 1,\quad 4A+6B+3C=-1$ <br>
$\Rightarrow{}\quad A = \frac{-2}{5},\quad B=\frac{3}{5},\quad C=-1$ <br>
$\Rightarrow{}\ \ \boxed{ \frac{x-1}{(3x+2)^2(2x+3)} = -\frac{2}{5(2x+3)} + \frac{3}{5(3x+2)} - \frac{1}{(3x+2)^2} }$
</div>

-----------------------------------------------------------------------------------

### Problem 2.
Obtain the derivative of the function, $f(x)=\frac{x+3}{2-x}$, using the definition of derivative (The limit of rise over run or "$\lim{(RoR)}$"
<div class = "answer">$\Rightarrow{}\quad$ using the expression $$f'(x) = \lim_{\Delta x\to0} \frac{f(x+\Delta x) - f(x)}{\Delta x}$$ <br>
$\Rightarrow{}\ \ f'(x) = \lim_{\Delta x\to0} \frac{\frac{(x+\Delta x)+3}{2-(x+\Delta x)} - \frac{(x+3)}{(2-x)}}{\Delta x} = \lim_{\Delta x\to0} \frac{\frac{5\Delta x}{(2-x)(2-x-\Delta x)}}{\Delta x}$ <br>
$\Rightarrow{}\ \ f'(x) = \lim_{\Delta x\to0} \frac{5}{(2-x)(2-x-\Delta x)}= \boxed{ \frac{5}{(2-x)^2} }$
</div>

-----------------------------------------------------------------------------------

### Problem 3.
Obtain the derivative of the following functions, using the product, chain and sum rule

(a) $f(x) = x^3 e^{2x}$
<div class = "answer">$\Rightarrow{}$ Using product rule $\Rightarrow{} \frac{d}{dx}(uv) = v\frac{du}{dx} + u\frac{dv}{dx}\\ \Rightarrow{} u = x^3,\quad v=\exp{(2x)}$ <br>
$\Rightarrow{} \frac{du}{dx} = 3x^2$ <br>
$\Rightarrow{}$ using chain rule $\frac{d}{dx}v(g(x)) = \frac{dv}{dg}\frac{dg}{dx}$ to solve $\frac{dv}{dx}$ with $g(x) = 2x $ <br>
$\Rightarrow{} \frac{dv}{dx} = 2\exp{(2x)}$ <br>
$\Rightarrow{} \boxed{\frac{df(x)}{dx} = 3x^2\exp{(2x)} + 2x^3\exp{(2x)} \Rightarrow{} \frac{df(x)}{dx} = x^2\exp{(2x)}(3 + 2x)}$
</div>

(b) $f(x) = \sin{(x^2 + 3x)}$
<div class = "answer">$\Rightarrow{}$ Using chain rule $\Rightarrow{} \frac{df(x)}{dx}= \cos{(x^2+3x)}\frac{d}{dx}(x^2+3x)$ <br>
$\Rightarrow{}$ Using sum rule $\Rightarrow{} \frac{d}{dx}(g(x)+h(x)) = \frac{dg}{dx} + \frac{dh}{dx}$ <br>
$\Rightarrow{} \frac{d}{dx}(x^2+3x) = 2x + 3 $ <br>
$\Rightarrow{} \boxed{\frac{df(x)}{dx} = \cos{(x^2+3x)}(2x + 3)}$
</div>

(c) $f(x) = \frac{x^2+2}{3x+1}$
<div class = "answer">$\Rightarrow{}$ Using product, chain and sum rule <br>
$\Rightarrow{} f(x) = (x^2+2)(3x+1)^{-1}$ <br>
$\Rightarrow{} \frac{df(x)}{dx} = 2x(3x+1)^{-1} + (x^2+2)(-3(3x+1)^{-2})$ <br>
$\Rightarrow{} \boxed{\frac{df(x)}{dx} = \frac{3x^2+2x-6}{(3x+1)^{2}}}$ <br>
</div>

-----------------------------------------------------------------------------------

### Problem 4.
Integrate the following functions, using the power rule, sum rule and integration by parts.

(a) $f(x) = 2x\sin{(x)}$
<div class = "answer">$\Rightarrow{} \int{2x\sin{(x)}}dx$ <br>
$\Rightarrow{}$ using integration by parts $\Rightarrow{} \int{udv} = uv -\int{vdu}$ <br>
$\Rightarrow{} u =2x,\quad dv=\sin{(x)dx} \Rightarrow{} du=2dx,\quad v=-\cos{(x)}$ <br>
$\Rightarrow{} \int{2x\sin{(x)}}dx = 2x(-\cos{(x)}) - \int{(-cox(x))2}dx$ <br>
$\Rightarrow{} \int{2x\sin{(x)}}dx = -2x\cos{(x)} + 2\int{\cos{(x)}}dx$ <br>
$\Rightarrow{} \boxed{\int{2x\sin{(x)}}dx = -2x\cos{(x)} + 2\sin{(x)} + c}$
</div>

(b) $f(x) = x^2 \ln{(4x)}$
<div class = "answer">$\Rightarrow{} \int{x^2 \ln{(4x)}}dx$ <br>
$\Rightarrow{}$ using integration by parts $\Rightarrow{} u =\ln{(4x)},\quad dv=x^2dx \Rightarrow{} du=\frac{1}{x}dx,\quad v=\frac{x^3}{3}$ <br>
$\Rightarrow{} \int{x^2 \ln{(4x)}}dx = \ln{(4x)}\frac{x^3}{3} - \int{\frac{x^3}{3}\frac{1}{x}}dx$ <br>
$\Rightarrow{} \int{x^2 \ln{(4x)}}dx = \frac{x^3}{3}\ln{(4x)} - \int{\frac{x^2}{3}}dx$ <br>
$\Rightarrow{} \int{x^2 \ln{(4x)}}dx = \frac{x^3}{3}\ln{(4x)} - \int{\frac{x^2}{3}}dx$ <br>
$\Rightarrow{} \int{x^2 \ln{(4x)}}dx = \frac{x^3}{3}\ln{(4x)} - \frac{x^3}{9} + c$ <br>
$\Rightarrow{} \boxed{\int{x^2 \ln{(4x)}}dx = \frac{x^3}{9}{(3\ln{(4x)} - 1) + c}}$ <br>
</div>

(c) $f(x) = x^5 e^{x^2}$
<div class = "answer">$\Rightarrow{} \int{x^5 \exp{(x^2)}}dx$ <br>
$\Rightarrow{}$ substitute $ u =x^2,\quad du=2xdx$ <br>
$\Rightarrow{} \int{x^5 \exp{(x^2)}}dx = \frac{1}{2}\int{u^2 \exp{(u)}}du$ <br>
$\Rightarrow{}$ using integration by parts <br>
$\Rightarrow{} f =u^2,\quad dg=\exp{(u)}du \\ \Rightarrow{} df=2udu,\quad g=\exp{(u)}$ <br>
$\Rightarrow{} \frac{1}{2}\int{u^2 \exp{(u)}}du = \frac{1}{2} \big[u^2\exp{(u)} - \int{\exp{(u)}2u}du \big]$ <br>
$\Rightarrow{} \frac{1}{2}\int{u^2 \exp{(u)}}du = \frac{1}{2}u^2\exp{(u)} - \int{\exp{(u)}u}du$ <br>
$\Rightarrow{}$ using integration by parts $\Rightarrow{} f =u,\quad dg=\exp{(u)}du \Rightarrow{} df=du,\quad g=\exp{(u)}$ <br>
$\Rightarrow{} \frac{1}{2}\int{u^2 \exp{(u)}}du = \frac{1}{2}u^2\exp{(u)} - \big[ u\exp{(u)} - \int{\exp{(u)}}du \big]$ <br>
$\Rightarrow{} \frac{1}{2}\int{u^2 \exp{(u)}}du = \frac{1}{2}u^2\exp{(u)} - u\exp{(u)} + \exp{(u)} + c$ <br>
$\Rightarrow{} \frac{1}{2}\int{u^2 \exp{(u)}}du = \frac{1}{2}\exp{(u)}(u^2 - 2u + 2) + c$ <br>
$\Rightarrow{}$ substitute back for $ u =x^2$ <br>
$\Rightarrow{} \boxed{\int{x^5 \exp{(x^2)}}dx = \frac{1}{2}\exp{(x^2)}(x^4 - 2x^2 + 2) + c}$
</div>

-----------------------------------------------------------------------------------

### Problem 5.
Express the following without logarithms (assume we are working in base 10 unless otherwise stated)

(a) $\log{x}=\log{P}+2\log{Q}-\log{K}-3$
<div class = "answer">$\log{x}=\log{\frac{PQ^2}{K}}-\log{1000\ \ \ }$ <br>
$\Rightarrow{}\ \ \boxed{=\frac{PQ^2}{1000K}}$ 
</div>

(b) $\log{R}=1+\frac{1}{3}\log{M}+3\log{S}$
<div class = "answer">$\Rightarrow{} \log{R=\log{10+\log{M^{\frac{1}{3}}+\log{S^3\ \ }}}}$ <br>
$\Rightarrow{}\ \boxed{R=10 \cdot S^3 \cdot \sqrt[3]{M}}$
</div>

(c) $\ln{P}=\frac{1}{2}\ln\left(Q+1\right)-3\ln{R}+2$
<div class = "answer">$\Rightarrow{} \ln{P=\ln{ \left(Q+1\right) }^{\frac{1}{2}}+\ln{e^2-\ln{R^3}}}$ <br>
$\Rightarrow{}\ \ \boxed{P=\frac{e^2\sqrt{Q+1}}{R^3}}$
</div>

-----------------------------------------------------------------------------------

### Problem 6.
Express the following in log form, with no fractions or powers inside the log.

(a) $V=\frac{\pi{}h}{4}\left(D-h\right)\left(D+h\right)$
<div class = "answer">$\Rightarrow\log{V=\boxed{\log{\pi{}+\log{h+\log{(D-h)}}}+\log{\left(D+h\right)-\log4}}}$</div>

(b) $P=\frac{1}{16}(2d-1)^2N\sqrt{S}$
<div class = "answer">$\Rightarrow\log{P}=\boxed{2\log{\left(2d-1\right)}+\log{N}+\frac{1}{2}\log{S}-\log{16}}$</div>

-----------------------------------------------------------------------------------

### Problem 7.
Solve the following equations using logarithm theorems.

(a) $\log{(5x-1)}=2$
<div class = "answer">${10}^2=5x-1\ \ \
\Rightarrow{}\ \ \ \boxed{x=\frac{101}{5}=20.2}$
</div>

(b) $\log_2{(x+1)}-\log_2{(x-4)}=3$
<div class = "answer">$\log_2{\frac{x+1}{x-4}}=3\ \ \ \Rightarrow{}\ \ \ 2^3=\frac{x+1}{x-4}$
$\Rightarrow{}\ \ \ x+1=8x-32\ \ \ \Rightarrow{}\ \ \ \boxed{x=\frac{33}{7}=4.71...}$
</div>

(c) $\log_6{(x+4)}+\log_6{(x-2)}=\log_6{(4x)}$ where $x>0$
<div class = "answer">$\log_6{\left((x+4).(x-2)\right)}=\log_6{4x}\ \ \Rightarrow{}\ \left(x+4\right)\left(x-2\right)=4x$ <br>
$\Rightarrow{}\ \ x^2-2x-8=0$ <br>
$\Rightarrow{}\ \ \ (x-4)(x+2)=0\ \ \ x_1=4 \text{ and } x_2=-2\ \ \ \Rightarrow{}\ \ \ \boxed{x=4}$
</div>

-----------------------------------------------------------------------------------

### Problem 8.
Determine the domain and range of the functions defined below.

(a) $f(x)=\cos^2{(x)}$
<div class = "answer">$\Rightarrow{}\boxed{
\text{Domain of } f\left(x\right)\ \Rightarrow{}\ \ (-\infty{},\infty{})}$ <br>
$\Rightarrow{} \boxed{ \text{Range of f }\left(x\right)\Rightarrow{}[0,1].}$
</div>

(b) $f(x)={-x}^2+5x-6$
<div class = "answer">$\Rightarrow{}\boxed{\text{Domain of f}\left(x\right)\ \Rightarrow{}\ \ (-\infty{},\infty{})}$ <br>
$\Rightarrow{}\boxed{\text{Range of } f(x) \Rightarrow{} \text{, function has one maximum.}
\Rightarrow{}\quad y\leq \frac{1}{4}}$
</div>

(c) $f(x)=-x^3+4x^2-4x\ $
<div class = "answer">$\Rightarrow{}\boxed{\text{
Domain of f}\left(x\right)\ \Rightarrow{}(-\infty{},\infty{})}$. <br>
$\Rightarrow{}\boxed{\text{Range of f}\left(x\right)\Rightarrow{}\ \ (-\infty{},\infty{})}$
</div>

(d) $f\left(x\right)=$exp⁡$(1/x)$
<div class = "answer">$y=e^{\frac{1}{x}}\ \Rightarrow{}$ at  $x=0$, the function is undefined.
$\Rightarrow{} \boxed{\text{Domain of } f(x)\ \Rightarrow{}(-\infty{},0)\cup{}(0,\infty{})}$. <br>
$y=e^{\frac{1}{x}}\ \Rightarrow{}$ at $y=1$, the function is undefined. <br>
$\Rightarrow{} 0 < y < 1 \text{ & } y>1$ <br>
$ \Rightarrow{}\ \ \boxed{\text{Range of } f(x)\ \Rightarrow{}\ \ (0,1)\cup{}(1,\infty{})}$</div>

(e) $f\left(x\right)=\frac{1}{e^x+1}$
<div class = "answer"> $\Rightarrow{} \boxed{\text{Domain of the function} \Rightarrow{}(-\infty{},\infty{})}$. <br>
$y=\frac{1}{e^x+1}\ \Rightarrow{}$ at $y=0\ \text{ & } y=1$, the function is undefined. <br>
$\Rightarrow{}\boxed{\text{Range of } f(x)\ \Rightarrow{}\ \ (0,1)}$.</div>

-----------------------------------------------------------------------------------

### Problem 9.
Evaluate the following by applying change of base to base 10 (rounded to 1 decimal place) and then using these numbers with finite accuracy to calculate the final answer (also to 3 significant figures)

(a) $\log_2{15}$
<div class = "answer">$\log_{10}2\times{}\log_2{15}=\log_{10}{15}$
$\Rightarrow{} \boxed{\log_2{15}=\frac{\log_{10}{15}}{\log_{10}2}\approx\frac{1.2}{0.3}=4.00.}$
</div>

(b) $\log_{20}{17}$
<div class = "answer">$\log_{10}20\times{}\log_{20}{17}=\log_{10}{17}$
$\Rightarrow{} \boxed{\log_{20}{17}=\frac{\log_{10}{17}}{\log_{10}20}\approx\frac{1.2}{1.3}=0.923}$
</div>

(c) $\log_3{16}$
<div class = "answer">$\log_{10}3\times{}\log_3{16}=\log_{10}{16}$ 
$\Rightarrow{} \boxed{\log_3{16}=\frac{\log_{10}{16}}{\log_{10}3}\approx\frac{1.2}{0.5}=2.40}$
</div>

## Exam Style Questions
### Problem 10.
[13 marks] A curve has equation $f(x) = \frac{ax^2 - 12}{4x^2 + bx - 6}$, where $a$ and $b$ are constants.

(a) Find the coordinates of the point where the curve crosses the $y$-axis

<div class = "answer"> When $x=0, f(x)=\frac{-12}{-6} \\ \Rightarrow{} f(x) = 2,\ \\ \Rightarrow{} \boxed{(0,2)}$ [1 mark]</div>

(b) You are given that the curve has a vertical asymptote at $x=2$. Find the value of $b$ and the equation of the other vertical asymptote.

<div class = "answer">At $x=2, 4x^2 +bx - 6 = 0$ <br>
$\Rightarrow 4(2)^2 + b(2) - 6 = 0 \Rightarrow \boxed{b = - 5}$ <br>
$\Rightarrow$ Factorise $4x^2 - 5x - 6$ <br>
$\Rightarrow (4x+3)(x-2)$  <br>
$\therefore$ The other asymptote occurs when $4x+3=0 \Rightarrow \boxed{x = -\frac{3}{4}}$
[3 marks]</div>

(c) You are given that the curve crosses the $x$-axis when $x= \pm{\sqrt{6}}$. Find the value of $a$ and the equation of the horizontal asymptote.

<div class = "answer">When $f(x)=0, x = \pm{\sqrt{6}}$ <br>
$\therefore 0 = \frac{ax^2 - 12}{4x^2 + bx - 6}\\ a(6)-12 = 0 $ <br>
$6a = 12 \Rightarrow \boxed{a = 2}$ <br>
Horizontal asymptote occurs when $x \rightarrow{\infty}$ <br>
$f(x)$ will tend to the highest powers of x <br>
$\Rightarrow f(x) = \frac{ax^2}{4x^2}$ <br>
Therefore, the horizontal asymptote occurs at $\boxed{y=\frac{1}{2}.}$ 
[2 marks]</div>

(d) Find the set of values for which $y \geqslant 0$.

<div class = "answer">Using the graph you sketched, you can see that $y$ is greater than or equal to zero in the regions where $\boxed{x\leqslant -\sqrt{6}, \space - \frac{3}{4} < x < 2, \space x \geqslant \sqrt{6}}$ [3 marks]
</div>

(e) Find the domain (using the set notation)

<div class = "answer">$\boxed{ x \ \epsilon \ \mathbb{R}, x \neq -\frac{3}{4}, x \neq 2}$
</div>

(f) Sketch the function, indicating the location of the features listed above

<div class = "answer"><iframe src="https://www.desmos.com/calculator/ll5ygltnd3?embed" width="500px" height="500px" style="border: 1px solid #ccc" frameborder=0></iframe>
</div>

-----------------------------------------------------------------------------------

### Problem 11.
[12 marks] A curve has equation $y=\frac{3x^2 - 9}{x^2 + 3x - 4}$

(a) Find the equations of the two vertical asymptotes and the one horizontal asymptote of this curve.

<div class = "answer">$\boxed{x = 1 \\ x = -4 \\ y = 3}$ [3 marks]</div>

(b) State, with justification, how the curve approaches the horizontal asymptote for large positive and large negative values of x.

<div class = "answer">$\text{Large positive}\ x, \boxed{y \ \rightarrow{3} \text{ from below}}$ <br>
$\text{Large negative} \ x, \boxed{ \ y \rightarrow{3}\text{ from above}}$</div>

(c) Sketch the curve

<div class = "answer"><iframe src="https://www.desmos.com/calculator/jdzogmrkh8?embed" width="500px" height="500px" style="border: 1px solid #ccc" frameborder=0> [3 marks]</iframe></div>

(d) Solve the inequality $\frac{3x^2 - 9}{x^2 + 3x -4} \geqslant 0. $

<div class = "answer">From the graph you have just sketched, you can see that the function is greater than or equal to zero in the regions where $\boxed{x<-4, -\sqrt{3} \leqslant x < 1, x \geqslant \sqrt{3}}$
[3 marks]</div>

------------
<button type="button" onclick="displayAnswerButtons('block')">Show answer buttons</button>
<button type="button" onclick="displayAnswers('block')">Show all answers</button>
<button type="button" onclick="displayAnswers('none')">Hide all answers</button>

<br><br>

# Next week, Vectors!
