<script type="text/x-mathjax-config">
  MathJax.Hub.Config({
    tex2jax: {
      inlineMath: [ ['$','$'], ["\\(","\\)"] ],
      processEscapes: true
    }
  });
</script>

<script type="text/javascript" async
  src="https://cdnjs.cloudflare.com/ajax/libs/mathjax/2.7.5/MathJax.js?config=TeX-MML-AM_CHTML">
</script>
<script type="text/javascript" src="tutorialSheetScripts.js"> </script>
<link rel="stylesheet" type="text/css" media="all" href="styles.css">

# Partial Differential Equations Tutorial Sheet, # 12

### Learning Targets
 * Evaluate and manipulate Partial Differentials
 * Understand how partial differentials work on vector fields
 * Use separation of variables solution to solve a PDE

### Additional resources
* [PDE intro video](https://youtu.be/PTvvoVLzVCE)

<br><br><br><br>

# Problem sheet
## Essential Questions
### Problem 1.
Which of the following are solutions to Laplace's equation,
$\nabla^2 f(\mathbf{x}) = 0$?
For those that are not, can you come up with a differential equation involving the Laplacian, $\nabla^2$, that $f(\mathbf{x})$ is a solution of?

(a) $e^{-y} \sin x $
<div class = "answer">
Yes, $\nabla^2 f(\mathbf{x}) = 0$
</div>

(b) $\sin\left(\frac{x+y}{2}\right)\sin\left(\frac{x-y}{2}\right)$
<div class = "answer">
No, but e.g. $\nabla^2 f(\mathbf{x}) + f = 0$
</div>

(c) $f(x + i y)$
<div class = "answer">
Yes, $\nabla^2 f(x + i y) = 0$, this becomes a useful result in complex analysis.
</div>

(d) $4 \arctan(y/x) + \log(x^2 +y^2)$
<div class = "answer">
Yes, $\nabla^2 f(\mathbf{x}) = 0$
</div>

(e) $\frac{x+y}{z}$
<div class = "answer">
No, but e.g. $\nabla^2 f(\mathbf{x}) = 2 f / z^2$ would work.
</div>

-----------------------------------------------------------------------------------

### Problem 2.
Show that the function $u\left(x,y\right)=\ln⁡(1+xy^2)$ satisfies the partial differential equation:

$$
2 \frac{\partial{} ^2u}{ \partial{} x^2} + 
y^3 \frac{ \partial{} ^2u }{ \partial{} y \partial{} x }
= 0
$$

<div class = "answer">
$$
\frac{\partial{}u}{\partial{}x}=\frac{y^2}{1+xy^2}\ ;\ \ \
\frac{ {\partial{}}^2u}{ {\partial{}x}^2}=-\frac{y^2}{ {\left(1+{xy}^2\right)}^2}.y^2=\frac{-y^4}{ {\left(1+{xy}^2\right)}^2}
$$
<br>

$$
\frac{ {\partial{}}^2u}{\partial{}y\partial{}x}=\frac{\partial{}}{\partial{}y}\left(\frac{\partial{}u}{\partial{}x}\right)=\frac{2y\left(1+xy^2\right)-y^2(2xy)}{ {(1+xy^2)}^2}=\frac{2y+2xy^3-2xy^3}{ { {(1+xy}^2)}^2}=\frac{2y}{ { {(1+xy}^2)}^2}
$$
<br>

$$
2\frac{ {\partial{}}^2u}{\partial{}x^2}+y^3\frac{ {\partial{}}^2u}{\partial{}y\partial{}x}=-\frac{2y^4}{ { {(1+xy}^2)}^2}+\frac{ {2y}^4}{ { {(1+xy}^2)}^2}=0
$$
</div>

-----------------------------------------------------------------------------------

### Problem 3.

Prove for the 1D diffusion equation,
$\frac{ \partial f(x,t)}{ \partial t} = \alpha \frac{ \partial^2 f(x,t)}{\partial x^2}$,
that the total area under the curve $f(x,t)$ does not change over time.
(You may assume that $\frac{ \partial f(x,t)}{ \partial x} \rightarrow 0$ for $x \rightarrow \pm\infty$).

<div class = "answer">
The area under the curve is calculated by integrating $f(x,t)$ over all x.
Integrating both sides of the PDE,

$$
\int_{-\infty}^{\infty} \mathrm{d}x \; \frac{ \partial {f(x,t)}}{ \partial t} = \int_{-\infty}^{\infty} \mathrm{d}x \; \alpha \frac{\partial f(x,t)}{\partial x}
$$

$\Rightarrow{}$ We can swap the order of differentiation and integration on the LHS and directly integrate the expression on the RHS,

$$
\frac{\partial}{\partial t} \int_{-\infty}^{\infty} \mathrm{d}x \; f(x,t) =
\alpha \left.\frac{ \partial f(x,t)}{ \partial x}\right| _ {x\rightarrow \infty} - \left.\alpha \frac{ \partial f(x,t)}{ \partial x}\right|_{x\rightarrow -\infty}
$$

$\Rightarrow{}$ The x derivatives go to zero at infinity

$$
\boxed{ \frac{\partial}{ \partial t} \int_{-\infty}^{\infty} \mathrm{d}x \; f(x,t) = 0 }
$$

$\Rightarrow{}$ Therefore the area under the concentration curve does not change in time.

The area will be proportional to numbers of ions or molecules etc. the total number of these will stay the same as they diffuse within the space.
The area taken over a region of the space will be proportional to the number of particles in that region.
</div>

-----------------------------------------------------------------------------------

### Problem 4.
Show that a Gaussian function,
$f(x,t) = \frac{1}{\sigma(t)\sqrt{2\pi}} \exp\left( -\frac{x^2}{2\sigma(t)^2} \right)$
, solves the 1D diffusion equation, on the condition that
$\sigma(t) = \sqrt{\sigma(0)^2 + 2 \alpha t}$.


<div class = "answer">
This is a show-that question, so you need only show it satisfies the equation, rather than proving it outright (which is done in the course notes). This is an ideal opportunity for the chain rule, rather than directly inserting the form of $\sigma(t)$. First calculate the derivatives of the diffusion equation:


\begin{align*}
\frac{\partial f(x,t)}{\partial t} &=
\frac{1}{\sqrt{2\pi}}\left[
-\frac{1}{\sigma(t)^2} + \frac{x^2}{\sigma(t)^4}
\right]\sigma'(t)\exp\left(-\frac{x^2}{2
\sigma(t)^2}\right)
\newline
\frac{\partial f(x,t)}{\partial x} &=
\frac{1}{\sqrt{2\pi}}\left[
-\frac{x}{\sigma(t)^3}
\right]\exp\left(-\frac{x^2}{2
\sigma(t)^2}\right)
\newline
\frac{\partial^2 f(x,t)}{\partial x^2} &=
\frac{1}{\sqrt{2\pi}}\left[
-\frac{1}{\sigma(t)^3}
+\frac{x^2}{\sigma(t)^5}
\right]\exp\left(-\frac{x^2}{2
\sigma(t)^2}\right)
\;,
\end{align*}

$\Rightarrow{}$ and then,

\begin{align*}
\sigma'(t) &= \frac{\alpha}{\sigma(0)^2 + 2 \alpha t} = \frac{\alpha}{\sigma(t)}
\;,
\end{align*}

$\Rightarrow{}$ Inserting into the diffusion equation,


\begin{align*}
\frac{f(x,t)}{t} &= \alpha \frac{ \partial^2 f(x,t)}{\partial x^2}
\newline
\frac{1}{\sqrt{2\pi}}\left[
-\frac{1}{\sigma(t)^2} + \frac{x^2}{\sigma(t)^4}
\right]\sigma'(t)\exp\left(-\frac{x^2}{2
\sigma(t)^2}\right)
&=
\alpha \frac{1}{\sqrt{2\pi}}\left[
-\frac{1}{\sigma(t)^3}
+\frac{x^2}{\sigma(t)^5}
\right]\exp\left(-\frac{x^2}{2
\sigma(t)^2}\right)
\end{align*}

$\Rightarrow{}$ Divide common terms,
\begin{align*}
\left[
-\frac{1}{\sigma(t)^2} + \frac{x^2}{\sigma(t)^4}
\right]\sigma'(t)
&=
\alpha \left[
-\frac{1}{\sigma(t)^3}
+\frac{x^2}{\sigma(t)^5}
\right]
\end{align*}

$\Rightarrow{}$ Substitute for $\sigma'(t)$,
\begin{align*}
\left[
-\frac{1}{\sigma(t)^2} + \frac{x^2}{\sigma(t)^4}
\right]
\frac{\alpha}{\sigma(t)}
&=
\alpha \left[
-\frac{1}{\sigma(t)^3}
+\frac{x^2}{\sigma(t)^5}
\right]
\end{align*}

$\Rightarrow{}$ LHS is equal RHS, so this is proven.
</div>

------------------------------

### Problem 5.

For an initial concentration,
$f(x,0) = \frac{1}{\sigma_0}\exp\left( -\frac{(x-x_0)^2}{2 \sigma_0^2} \right)$,
governed by the diffusion equation, calculate the concentration at
$x=0\,\mu\mathrm{m}$ and $t=10\,\mathrm{s}$, for $x_0 = 5\,\mu\mathrm{m}$,
$\sigma_0 = 1\,\mu\mathrm{m}$, and $\alpha = 2\,\mu\mathrm{m}^2\mathrm{s}^{-1}$.
(Use the solution given in Q4 to help)

<div class = "answer">
$\Rightarrow{}$ First set up a solution to the diffusion equation such that it matches the initial condition. i.e.

$$
f(x,t) = \frac{1}{\sqrt{\sigma_0^2 + 2 \alpha t}}
\exp\left(-\frac{(x-x0)^2}{2
{\sigma_0^2 + 4 \alpha t}}\right) \;.
$$

$\Rightarrow{}$ Then substitute in all constant and variable values,

$$
f(x=0,t=10\,\mathrm{s}) = \frac{1}{\sqrt{(1\,\mu\mathrm{m})^2 + 2\times2\,\mu\mathrm{m}^2\mathrm{s}^{-1} \, 10\,\mathrm{s}}}
\exp\left(-\frac{(0-5\,\mu\mathrm{m})^2}{2\times
{(1\,\mu\mathrm{m})^2 + 4 \times 2\,\mu\mathrm{m}^2\mathrm{s}^{-1} \, 10\,\mathrm{s}}}\right) \;
$$


$\Rightarrow{}$ Which reduces to,
$$
\boxed{ f(x=0,t=10\,\mathrm{s}) = \frac{1}{\sqrt{41\,\mu\mathrm{m}^2}}
\exp\left(-\frac{25\,\mu\mathrm{m}^2}{82\,\mu\mathrm{m}^2}\right)
\approx 0.12 \mu\mathrm{m}^{-1} }
$$
</div>

-----------------------------------

## Exam Style Questions
### Problem 6.

Solve the 3D wave equation by separation of variables to show,
$u(\mathbf{x}, t) = \exp(i\mathbf{k}\cdot\mathbf{x} - i \omega t)$,
is a solution. With $\mathbf{k} = (k_x, k_y, k_z)^T$
What is the resulting relationship between $\mathbf{k}$ and $\omega$?
$$
\frac{n^2}{c^2}\frac{\partial^2 u(\mathbf{x}, t)}{\partial t^2} - \nabla^2 u(\mathbf{x}, t) = 0
$$

<div class = "answer">
<b>NB:</b>   Coordinate vector $\mathbf{x} = (x,y,z)$ and, $u(\mathbf{x}) = (u(x),v(x),w(x))^T$ is a vector field. (Don’t forget the AT notation allows us to write a column vector as a transposed row vector, to save space!) <br><br>
    
$\Rightarrow{}$ Start with a separation of variables solution, let $u(\mathbf{x}, t) = X(x)Y(y)Z(z)T(t)$.
then,

\begin{align*}\frac{n^2}{c^2}{T''(t)}{X(x)Y(y)Z(z)} - \frac{X''(x)}{Y(y)Z(z)T(t)} - \frac{Y''(y)}{X(x)Z(z)T(t))} - \frac{Z''(z)}{X(x)Y(y)T(t)} = 0 \end{align*}
\begin{align*}
\frac{n^2}{c^2}\frac{T''(t)}{T(t)} - \frac{X''(x)}{X(x)} - \frac{Y''(y)}{Y(y)} - \frac{Z''(z)}{Z(z)} = 0
\end{align*}

$\Rightarrow{}$ There is some freedom of choice as to how you define the constants here.
In order to match to the test solution, $u(\mathbf{x}, t) = \exp(i\mathbf{k}\cdot\mathbf{x} - i \omega t)$,
the most straightforward choice is,

\begin{align*}
\frac{T''(t)}{T(t)} = -\omega^2 \quad
\frac{X''(x)}{X(x)} = -k_x^2 \quad
\frac{Y''(y)}{Y(y)} = -k_y^2 \quad
\frac{Z''(z)}{Z(z)} = -k_z^2 \space .
\end{align*}

$\Rightarrow{}$  But here we'll solve as if we assumed arbitrary constants instead,

\begin{align*}
\frac{T''(t)}{T(t)} = a \quad
\frac{X''(x)}{X(x)} = b \quad
\frac{Y''(y)}{Y(y)} = c \quad
\frac{Z''(z)}{Z(z)} = d \space .
\end{align*}

$\Rightarrow{}$ With $\frac{n^2}{c^2} a + b + c + d = 0$.
Solving the ODEs, we get,

\begin{align*}
T(t) &= A_+ e^{+ \sqrt{a} t} + A_- e^{- \sqrt{a} t}
\newline
X(x) &= B_+ e^{+ \sqrt{b} x} + B_- e^{- \sqrt{b} t}
\end{align*}

$\Rightarrow{}$ And equivalently for $Y(y)$ and $Z(z)$.
To match with our test solution,

$u(\mathbf{x}, t) = \exp(i\mathbf{k}\cdot\mathbf{x} - i \omega t)$, We'll keep the negative exponential from the $T(t)$ function,
and the positive exponentials from the spatial functions.
This allow us to build the solution,

$u(\mathbf{x}, t) \propto \exp(\sqrt{b} x + \sqrt{c} y + \sqrt{d} z - \sqrt{a} t)$,
Matching coefficients requires,}

$$
\sqrt{a} = i \omega \quad
\sqrt{b} = i k_x \quad
\sqrt{c} = i k_y \quad
\sqrt{d} = i k_z \quad .
$$

$\Rightarrow{}$ Which gives,
$u(\mathbf{x}, t) \propto \exp(i k_x x + i k_y y + i k_z z - i \omega t)$,
or $\exp(i\mathbf{k}\cdot\mathbf{x} - i \omega t)$.
and a dispersion relations,}

$$
\boxed{ \frac{n^2}{c^2} \omega^2 = k_x^2 + k_y^2 + k_z^2 }
$$

</div>


## Answers

<button type="button" onclick="displayAnswerButtons('block')">Show answer buttons</button>
<button type="button" onclick="displayAnswers('block')">Show all answers</button>
<button type="button" onclick="displayAnswers('none')">Hide all answers</button>

<br><br>

# Next week, Finite Methods!